src/normalization.lean
@@ -49,11 +49,10 @@ theorem semWfCons {Γ A k} (hΓ : ⊨ Γ) (hA : Γ ⊨ A ∶ 𝒰 k) : ⊨ Γ �
     exists rename succ k
     exact semWeaken (A := 𝒰 k) hB
 
-theorem soundness {w} (h : Wtf w) :
-  match w with
-  | ⟨.wf, Γ⟩ => ⊨ Γ
-  | ⟨.wt, ⟨Γ, a, A⟩⟩ => Γ ⊨ a ∶ A := by
-  induction h using wtfInd
+theorem soundness :
+  (∀ {Γ}, ⊢ Γ → ⊨ Γ) ∧
+  (∀ {Γ} {a A : Term}, Γ ⊢ a ∶ A → Γ ⊨ a ∶ A) := by
+  apply wtfInd <;> intros
   case nil => intro x A mem; cases mem
   case cons k _ _ hΓ hA => exact semWfCons hΓ hA
   all_goals intro σ hσ
@@ -190,7 +189,8 @@ theorem soundness {w} (h : Wtf w) :
 -----------------------------------*-/
 
 theorem normalization {Γ} {a A : Term} (h : Γ ⊢ a ∶ A) : wnf a ∧ wnf A := by
-  let ⟨_, _, hA, ha⟩ := soundness h var ?_
+  let ⟨_, ih⟩ := soundness
+  let ⟨_, _, hA, ha⟩ := ih h var ?_
   . rw [substId] at ha hA
     let ⟨_, CRnf⟩ := adequacy hA a
     exact ⟨CRnf ha, interpsWnf hA⟩
